Owl/owl.v
@@ -217,7 +217,8 @@ Fixpoint extRen_label {m_label : nat} {n_label : nat}
 (xi_label : fin m_label -> fin n_label)
 (zeta_label : fin m_label -> fin n_label)
 (Eq_label : forall x, xi_label x = zeta_label x) (s : label m_label) {struct
- s} : ren_label xi_label s = ren_label zeta_label s :=
+ s} :
+ren_label xi_label s = ren_label zeta_label s :=
   match s with
   | var_label _ s0 => ap (var_label n_label) (Eq_label s0)
   | latl _ s0 => congr_latl (eq_refl s0)
@@ -376,7 +377,8 @@ exact (fun n =>
                 (eq_sym
                    (compRenRen_label zeta_label shift
                       (funcomp shift zeta_label) (fun x => eq_refl)
-                      (sigma fin_n))) (ap (ren_label shift) (Eq fin_n)))
+                      (sigma fin_n)))
+                (ap (ren_label shift) (Eq fin_n)))
        | None => eq_refl
        end).
 Qed.
@@ -387,7 +389,8 @@ Lemma up_subst_ren_list_label_label {p : nat} {k : nat} {l_label : nat}
   (Eq : forall x, funcomp (ren_label zeta_label) sigma x = theta x) :
   forall x,
   funcomp (ren_label (upRen_list_label_label p zeta_label))
-    (up_list_label_label p sigma) x = up_list_label_label p theta x.
+    (up_list_label_label p sigma) x =
+  up_list_label_label p theta x.
 Proof.
 exact (fun n =>
        eq_trans (scons_p_comp' _ _ _ n)
@@ -403,7 +406,8 @@ exact (fun n =>
                   (eq_sym
                      (compRenRen_label zeta_label (shift_p p)
                         (funcomp (shift_p p) zeta_label) (fun x => eq_refl)
-                        (sigma n))) (ap (ren_label (shift_p p)) (Eq n)))))).
+                        (sigma n)))
+                  (ap (ren_label (shift_p p)) (Eq n)))))).
 Qed.
 
 Fixpoint compSubstRen_label {k_label : nat} {l_label : nat} {m_label : nat}
@@ -459,7 +463,8 @@ Lemma up_subst_subst_list_label_label {p : nat} {k : nat} {l_label : nat}
   (Eq : forall x, funcomp (subst_label tau_label) sigma x = theta x) :
   forall x,
   funcomp (subst_label (up_list_label_label p tau_label))
-    (up_list_label_label p sigma) x = up_list_label_label p theta x.
+    (up_list_label_label p sigma) x =
+  up_list_label_label p theta x.
 Proof.
 exact (fun n =>
        eq_trans
@@ -952,6 +957,8 @@ exact (fun s =>
        eq_ind_r (fun t => t = s) (instId'_constr s) (rinstInst'_constr id s)).
 Qed.
 
+Definition op := list binary -> Dist binary.
+
 Inductive tm (n_label n_tm : nat) : Type :=
   | var_tm : fin n_tm -> tm n_label n_tm
   | error : tm n_label n_tm
@@ -961,7 +968,7 @@ Inductive tm (n_label n_tm : nat) : Type :=
   | fixlam : tm n_label (S (S n_tm)) -> tm n_label n_tm
   | tlam : tm n_label n_tm -> tm n_label n_tm
   | l_lam : tm (S n_label) n_tm -> tm n_label n_tm
-  | op : tm n_label n_tm -> list (tm n_label n_tm) -> tm n_label n_tm
+  | Op : op -> list (tm n_label n_tm) -> tm n_label n_tm
   | zero : tm n_label n_tm -> tm n_label n_tm
   | app : tm n_label n_tm -> tm n_label n_tm -> tm n_label n_tm
   | alloc : tm n_label n_tm -> tm n_label n_tm
@@ -1030,13 +1037,12 @@ Proof.
 exact (eq_trans eq_refl (ap (fun x => l_lam m_label m_tm x) H0)).
 Qed.
 
-Lemma congr_op {m_label m_tm : nat} {s0 : tm m_label m_tm}
-  {s1 : list (tm m_label m_tm)} {t0 : tm m_label m_tm}
-  {t1 : list (tm m_label m_tm)} (H0 : s0 = t0) (H1 : s1 = t1) :
-  op m_label m_tm s0 s1 = op m_label m_tm t0 t1.
+Lemma congr_Op {m_label m_tm : nat} {s0 : op} {s1 : list (tm m_label m_tm)}
+  {t0 : op} {t1 : list (tm m_label m_tm)} (H0 : s0 = t0) (H1 : s1 = t1) :
+  Op m_label m_tm s0 s1 = Op m_label m_tm t0 t1.
 Proof.
-exact (eq_trans (eq_trans eq_refl (ap (fun x => op m_label m_tm x s1) H0))
-         (ap (fun x => op m_label m_tm t0 x) H1)).
+exact (eq_trans (eq_trans eq_refl (ap (fun x => Op m_label m_tm x s1) H0))
+         (ap (fun x => Op m_label m_tm t0 x) H1)).
 Qed.
 
 Lemma congr_zero {m_label m_tm : nat} {s0 : tm m_label m_tm}
@@ -1247,9 +1253,7 @@ Fixpoint ren_tm {m_label m_tm : nat} {n_label n_tm : nat}
   | l_lam _ _ s0 =>
       l_lam n_label n_tm
         (ren_tm (upRen_label_label xi_label) (upRen_label_tm xi_tm) s0)
-  | op _ _ s0 s1 =>
-      op n_label n_tm (ren_tm xi_label xi_tm s0)
-        (list_map (ren_tm xi_label xi_tm) s1)
+  | Op _ _ s0 s1 => Op n_label n_tm s0 (list_map (ren_tm xi_label xi_tm) s1)
   | zero _ _ s0 => zero n_label n_tm (ren_tm xi_label xi_tm s0)
   | app _ _ s0 s1 =>
       app n_label n_tm (ren_tm xi_label xi_tm s0) (ren_tm xi_label xi_tm s1)
@@ -1342,9 +1346,8 @@ tm n_label n_tm :=
   | l_lam _ _ s0 =>
       l_lam n_label n_tm
         (subst_tm (up_label_label sigma_label) (up_label_tm sigma_tm) s0)
-  | op _ _ s0 s1 =>
-      op n_label n_tm (subst_tm sigma_label sigma_tm s0)
-        (list_map (subst_tm sigma_label sigma_tm) s1)
+  | Op _ _ s0 s1 =>
+      Op n_label n_tm s0 (list_map (subst_tm sigma_label sigma_tm) s1)
   | zero _ _ s0 => zero n_label n_tm (subst_tm sigma_label sigma_tm s0)
   | app _ _ s0 s1 =>
       app n_label n_tm (subst_tm sigma_label sigma_tm s0)
@@ -1459,8 +1462,8 @@ Fixpoint idSubst_tm {m_label m_tm : nat}
       congr_l_lam
         (idSubst_tm (up_label_label sigma_label) (up_label_tm sigma_tm)
            (upId_label_label _ Eq_label) (upId_label_tm _ Eq_tm) s0)
-  | op _ _ s0 s1 =>
-      congr_op (idSubst_tm sigma_label sigma_tm Eq_label Eq_tm s0)
+  | Op _ _ s0 s1 =>
+      congr_Op (eq_refl s0)
         (list_id (idSubst_tm sigma_label sigma_tm Eq_label Eq_tm) s1)
   | zero _ _ s0 =>
       congr_zero (idSubst_tm sigma_label sigma_tm Eq_label Eq_tm s0)
@@ -1592,9 +1595,8 @@ ren_tm xi_label xi_tm s = ren_tm zeta_label zeta_tm s :=
            (upRen_label_label zeta_label) (upRen_label_tm zeta_tm)
            (upExtRen_label_label _ _ Eq_label) (upExtRen_label_tm _ _ Eq_tm)
            s0)
-  | op _ _ s0 s1 =>
-      congr_op
-        (extRen_tm xi_label xi_tm zeta_label zeta_tm Eq_label Eq_tm s0)
+  | Op _ _ s0 s1 =>
+      congr_Op (eq_refl s0)
         (list_ext
            (extRen_tm xi_label xi_tm zeta_label zeta_tm Eq_label Eq_tm) s1)
   | zero _ _ s0 =>
@@ -1752,9 +1754,8 @@ subst_tm sigma_label sigma_tm s = subst_tm tau_label tau_tm s :=
         (ext_tm (up_label_label sigma_label) (up_label_tm sigma_tm)
            (up_label_label tau_label) (up_label_tm tau_tm)
            (upExt_label_label _ _ Eq_label) (upExt_label_tm _ _ Eq_tm) s0)
-  | op _ _ s0 s1 =>
-      congr_op
-        (ext_tm sigma_label sigma_tm tau_label tau_tm Eq_label Eq_tm s0)
+  | Op _ _ s0 s1 =>
+      congr_Op (eq_refl s0)
         (list_ext
            (ext_tm sigma_label sigma_tm tau_label tau_tm Eq_label Eq_tm) s1)
   | zero _ _ s0 =>
@@ -1920,13 +1921,12 @@ ren_tm rho_label rho_tm s :=
            (upRen_label_label zeta_label) (upRen_label_tm zeta_tm)
            (upRen_label_label rho_label) (upRen_label_tm rho_tm)
            (up_ren_ren _ _ _ Eq_label) Eq_tm s0)
-  | op _ _ s0 s1 =>
-      congr_op
-        (compRenRen_tm xi_label xi_tm zeta_label zeta_tm rho_label rho_tm
-           Eq_label Eq_tm s0)
+  | Op _ _ s0 s1 =>
+      congr_Op (eq_refl s0)
         (list_comp
            (compRenRen_tm xi_label xi_tm zeta_label zeta_tm rho_label rho_tm
-              Eq_label Eq_tm) s1)
+              Eq_label Eq_tm)
+           s1)
   | zero _ _ s0 =>
       congr_zero
         (compRenRen_tm xi_label xi_tm zeta_label zeta_tm rho_label rho_tm
@@ -2136,13 +2136,12 @@ subst_tm theta_label theta_tm s :=
            (up_label_label theta_label) (up_label_tm theta_tm)
            (up_ren_subst_label_label _ _ _ Eq_label)
            (up_ren_subst_label_tm _ _ _ Eq_tm) s0)
-  | op _ _ s0 s1 =>
-      congr_op
-        (compRenSubst_tm xi_label xi_tm tau_label tau_tm theta_label theta_tm
-           Eq_label Eq_tm s0)
+  | Op _ _ s0 s1 =>
+      congr_Op (eq_refl s0)
         (list_comp
            (compRenSubst_tm xi_label xi_tm tau_label tau_tm theta_label
-              theta_tm Eq_label Eq_tm) s1)
+              theta_tm Eq_label Eq_tm)
+           s1)
   | zero _ _ s0 =>
       congr_zero
         (compRenSubst_tm xi_label xi_tm tau_label tau_tm theta_label theta_tm
@@ -2253,7 +2252,8 @@ Lemma up_subst_ren_label_tm {k : nat} {l_label l_tm : nat}
   (Eq : forall x, funcomp (ren_tm zeta_label zeta_tm) sigma x = theta x) :
   forall x,
   funcomp (ren_tm (upRen_label_label zeta_label) (upRen_label_tm zeta_tm))
-    (up_label_tm sigma) x = up_label_tm theta x.
+    (up_label_tm sigma) x =
+  up_label_tm theta x.
 Proof.
 exact (fun n =>
        eq_trans
@@ -2284,7 +2284,8 @@ exact (fun n =>
          (eq_trans
             (eq_sym
                (compRenRen_label zeta_label id (funcomp id zeta_label)
-                  (fun x => eq_refl) (sigma n))) (ap (ren_label id) (Eq n)))).
+                  (fun x => eq_refl) (sigma n)))
+            (ap (ren_label id) (Eq n)))).
 Qed.
 
 Lemma up_subst_ren_tm_tm {k : nat} {l_label l_tm : nat} {m_label m_tm : nat}
@@ -2294,7 +2295,8 @@ Lemma up_subst_ren_tm_tm {k : nat} {l_label l_tm : nat} {m_label m_tm : nat}
   (Eq : forall x, funcomp (ren_tm zeta_label zeta_tm) sigma x = theta x) :
   forall x,
   funcomp (ren_tm (upRen_tm_label zeta_label) (upRen_tm_tm zeta_tm))
-    (up_tm_tm sigma) x = up_tm_tm theta x.
+    (up_tm_tm sigma) x =
+  up_tm_tm theta x.
 Proof.
 exact (fun n =>
        match n with
@@ -2322,7 +2324,8 @@ Lemma up_subst_ren_list_label_tm {p : nat} {k : nat} {l_label l_tm : nat}
   forall x,
   funcomp
     (ren_tm (upRen_list_label_label p zeta_label)
-       (upRen_list_label_tm p zeta_tm)) (up_list_label_tm p sigma) x =
+       (upRen_list_label_tm p zeta_tm))
+    (up_list_label_tm p sigma) x =
   up_list_label_tm p theta x.
 Proof.
 exact (fun n =>
@@ -2345,7 +2348,8 @@ Lemma up_subst_ren_list_tm_label {p : nat} {k : nat} {l_label : nat}
   (Eq : forall x, funcomp (ren_label zeta_label) sigma x = theta x) :
   forall x,
   funcomp (ren_label (upRen_list_tm_label p zeta_label))
-    (up_list_tm_label p sigma) x = up_list_tm_label p theta x.
+    (up_list_tm_label p sigma) x =
+  up_list_tm_label p theta x.
 Proof.
 exact (fun n =>
        eq_trans
@@ -2354,7 +2358,8 @@ exact (fun n =>
          (eq_trans
             (eq_sym
                (compRenRen_label zeta_label id (funcomp id zeta_label)
-                  (fun x => eq_refl) (sigma n))) (ap (ren_label id) (Eq n)))).
+                  (fun x => eq_refl) (sigma n)))
+            (ap (ren_label id) (Eq n)))).
 Qed.
 
 Lemma up_subst_ren_list_tm_tm {p : nat} {k : nat} {l_label l_tm : nat}
@@ -2365,7 +2370,8 @@ Lemma up_subst_ren_list_tm_tm {p : nat} {k : nat} {l_label l_tm : nat}
   forall x,
   funcomp
     (ren_tm (upRen_list_tm_label p zeta_label) (upRen_list_tm_tm p zeta_tm))
-    (up_list_tm_tm p sigma) x = up_list_tm_tm p theta x.
+    (up_list_tm_tm p sigma) x =
+  up_list_tm_tm p theta x.
 Proof.
 exact (fun n =>
        eq_trans (scons_p_comp' _ _ _ n)
@@ -2427,13 +2433,12 @@ subst_tm theta_label theta_tm s :=
            (up_label_label theta_label) (up_label_tm theta_tm)
            (up_subst_ren_label_label _ _ _ Eq_label)
            (up_subst_ren_label_tm _ _ _ _ Eq_tm) s0)
-  | op _ _ s0 s1 =>
-      congr_op
-        (compSubstRen_tm sigma_label sigma_tm zeta_label zeta_tm theta_label
-           theta_tm Eq_label Eq_tm s0)
+  | Op _ _ s0 s1 =>
+      congr_Op (eq_refl s0)
         (list_comp
            (compSubstRen_tm sigma_label sigma_tm zeta_label zeta_tm
-              theta_label theta_tm Eq_label Eq_tm) s1)
+              theta_label theta_tm Eq_label Eq_tm)
+           s1)
   | zero _ _ s0 =>
       congr_zero
         (compSubstRen_tm sigma_label sigma_tm zeta_label zeta_tm theta_label
@@ -2544,7 +2549,8 @@ Lemma up_subst_subst_label_tm {k : nat} {l_label l_tm : nat}
   (Eq : forall x, funcomp (subst_tm tau_label tau_tm) sigma x = theta x) :
   forall x,
   funcomp (subst_tm (up_label_label tau_label) (up_label_tm tau_tm))
-    (up_label_tm sigma) x = up_label_tm theta x.
+    (up_label_tm sigma) x =
+  up_label_tm theta x.
 Proof.
 exact (fun n =>
        eq_trans
@@ -2577,7 +2583,8 @@ exact (fun n =>
             (eq_sym
                (compSubstRen_label tau_label id
                   (funcomp (ren_label id) tau_label) (fun x => eq_refl)
-                  (sigma n))) (ap (ren_label id) (Eq n)))).
+                  (sigma n)))
+            (ap (ren_label id) (Eq n)))).
 Qed.
 
 Lemma up_subst_subst_tm_tm {k : nat} {l_label l_tm : nat}
@@ -2587,7 +2594,8 @@ Lemma up_subst_subst_tm_tm {k : nat} {l_label l_tm : nat}
   (Eq : forall x, funcomp (subst_tm tau_label tau_tm) sigma x = theta x) :
   forall x,
   funcomp (subst_tm (up_tm_label tau_label) (up_tm_tm tau_tm))
-    (up_tm_tm sigma) x = up_tm_tm theta x.
+    (up_tm_tm sigma) x =
+  up_tm_tm theta x.
 Proof.
 exact (fun n =>
        match n with
@@ -2616,7 +2624,8 @@ Lemma up_subst_subst_list_label_tm {p : nat} {k : nat} {l_label l_tm : nat}
   forall x,
   funcomp
     (subst_tm (up_list_label_label p tau_label) (up_list_label_tm p tau_tm))
-    (up_list_label_tm p sigma) x = up_list_label_tm p theta x.
+    (up_list_label_tm p sigma) x =
+  up_list_label_tm p theta x.
 Proof.
 exact (fun n =>
        eq_trans
@@ -2639,7 +2648,8 @@ Lemma up_subst_subst_list_tm_label {p : nat} {k : nat} {l_label : nat}
   (Eq : forall x, funcomp (subst_label tau_label) sigma x = theta x) :
   forall x,
   funcomp (subst_label (up_list_tm_label p tau_label))
-    (up_list_tm_label p sigma) x = up_list_tm_label p theta x.
+    (up_list_tm_label p sigma) x =
+  up_list_tm_label p theta x.
 Proof.
 exact (fun n =>
        eq_trans
@@ -2649,7 +2659,8 @@ exact (fun n =>
          (eq_trans
             (eq_sym
                (compSubstRen_label tau_label id _ (fun x => eq_sym eq_refl)
-                  (sigma n))) (ap (ren_label id) (Eq n)))).
+                  (sigma n)))
+            (ap (ren_label id) (Eq n)))).
 Qed.
 
 Lemma up_subst_subst_list_tm_tm {p : nat} {k : nat} {l_label l_tm : nat}
@@ -2659,7 +2670,8 @@ Lemma up_subst_subst_list_tm_tm {p : nat} {k : nat} {l_label l_tm : nat}
   (Eq : forall x, funcomp (subst_tm tau_label tau_tm) sigma x = theta x) :
   forall x,
   funcomp (subst_tm (up_list_tm_label p tau_label) (up_list_tm_tm p tau_tm))
-    (up_list_tm_tm p sigma) x = up_list_tm_tm p theta x.
+    (up_list_tm_tm p sigma) x =
+  up_list_tm_tm p theta x.
 Proof.
 exact (fun n =>
        eq_trans
@@ -2724,13 +2736,12 @@ subst_tm theta_label theta_tm s :=
            (up_label_tm tau_tm) (up_label_label theta_label)
            (up_label_tm theta_tm) (up_subst_subst_label_label _ _ _ Eq_label)
            (up_subst_subst_label_tm _ _ _ _ Eq_tm) s0)
-  | op _ _ s0 s1 =>
-      congr_op
-        (compSubstSubst_tm sigma_label sigma_tm tau_label tau_tm theta_label
-           theta_tm Eq_label Eq_tm s0)
+  | Op _ _ s0 s1 =>
+      congr_Op (eq_refl s0)
         (list_comp
            (compSubstSubst_tm sigma_label sigma_tm tau_label tau_tm
-              theta_label theta_tm Eq_label Eq_tm) s1)
+              theta_label theta_tm Eq_label Eq_tm)
+           s1)
   | zero _ _ s0 =>
       congr_zero
         (compSubstSubst_tm sigma_label sigma_tm tau_label tau_tm theta_label
@@ -3034,9 +3045,8 @@ ren_tm xi_label xi_tm s = subst_tm sigma_label sigma_tm s :=
            (up_label_label sigma_label) (up_label_tm sigma_tm)
            (rinstInst_up_label_label _ _ Eq_label)
            (rinstInst_up_label_tm _ _ Eq_tm) s0)
-  | op _ _ s0 s1 =>
-      congr_op
-        (rinst_inst_tm xi_label xi_tm sigma_label sigma_tm Eq_label Eq_tm s0)
+  | Op _ _ s0 s1 =>
+      congr_Op (eq_refl s0)
         (list_ext
            (rinst_inst_tm xi_label xi_tm sigma_label sigma_tm Eq_label Eq_tm)
            s1)
@@ -4022,7 +4032,8 @@ Lemma up_subst_ren_label_ty {k : nat} {l_label l_ty : nat}
   (Eq : forall x, funcomp (ren_ty zeta_label zeta_ty) sigma x = theta x) :
   forall x,
   funcomp (ren_ty (upRen_label_label zeta_label) (upRen_label_ty zeta_ty))
-    (up_label_ty sigma) x = up_label_ty theta x.
+    (up_label_ty sigma) x =
+  up_label_ty theta x.
 Proof.
 exact (fun n =>
        eq_trans
@@ -4053,7 +4064,8 @@ exact (fun n =>
          (eq_trans
             (eq_sym
                (compRenRen_label zeta_label id (funcomp id zeta_label)
-                  (fun x => eq_refl) (sigma n))) (ap (ren_label id) (Eq n)))).
+                  (fun x => eq_refl) (sigma n)))
+            (ap (ren_label id) (Eq n)))).
 Qed.
 
 Lemma up_subst_ren_ty_ty {k : nat} {l_label l_ty : nat} {m_label m_ty : nat}
@@ -4063,7 +4075,8 @@ Lemma up_subst_ren_ty_ty {k : nat} {l_label l_ty : nat} {m_label m_ty : nat}
   (Eq : forall x, funcomp (ren_ty zeta_label zeta_ty) sigma x = theta x) :
   forall x,
   funcomp (ren_ty (upRen_ty_label zeta_label) (upRen_ty_ty zeta_ty))
-    (up_ty_ty sigma) x = up_ty_ty theta x.
+    (up_ty_ty sigma) x =
+  up_ty_ty theta x.
 Proof.
 exact (fun n =>
        match n with
@@ -4091,7 +4104,8 @@ Lemma up_subst_ren_list_label_ty {p : nat} {k : nat} {l_label l_ty : nat}
   forall x,
   funcomp
     (ren_ty (upRen_list_label_label p zeta_label)
-       (upRen_list_label_ty p zeta_ty)) (up_list_label_ty p sigma) x =
+       (upRen_list_label_ty p zeta_ty))
+    (up_list_label_ty p sigma) x =
   up_list_label_ty p theta x.
 Proof.
 exact (fun n =>
@@ -4114,7 +4128,8 @@ Lemma up_subst_ren_list_ty_label {p : nat} {k : nat} {l_label : nat}
   (Eq : forall x, funcomp (ren_label zeta_label) sigma x = theta x) :
   forall x,
   funcomp (ren_label (upRen_list_ty_label p zeta_label))
-    (up_list_ty_label p sigma) x = up_list_ty_label p theta x.
+    (up_list_ty_label p sigma) x =
+  up_list_ty_label p theta x.
 Proof.
 exact (fun n =>
        eq_trans
@@ -4123,7 +4138,8 @@ exact (fun n =>
          (eq_trans
             (eq_sym
                (compRenRen_label zeta_label id (funcomp id zeta_label)
-                  (fun x => eq_refl) (sigma n))) (ap (ren_label id) (Eq n)))).
+                  (fun x => eq_refl) (sigma n)))
+            (ap (ren_label id) (Eq n)))).
 Qed.
 
 Lemma up_subst_ren_list_ty_ty {p : nat} {k : nat} {l_label l_ty : nat}
@@ -4134,7 +4150,8 @@ Lemma up_subst_ren_list_ty_ty {p : nat} {k : nat} {l_label l_ty : nat}
   forall x,
   funcomp
     (ren_ty (upRen_list_ty_label p zeta_label) (upRen_list_ty_ty p zeta_ty))
-    (up_list_ty_ty p sigma) x = up_list_ty_ty p theta x.
+    (up_list_ty_ty p sigma) x =
+  up_list_ty_ty p theta x.
 Proof.
 exact (fun n =>
        eq_trans (scons_p_comp' _ _ _ n)
@@ -4239,7 +4256,8 @@ Lemma up_subst_subst_label_ty {k : nat} {l_label l_ty : nat}
   (Eq : forall x, funcomp (subst_ty tau_label tau_ty) sigma x = theta x) :
   forall x,
   funcomp (subst_ty (up_label_label tau_label) (up_label_ty tau_ty))
-    (up_label_ty sigma) x = up_label_ty theta x.
+    (up_label_ty sigma) x =
+  up_label_ty theta x.
 Proof.
 exact (fun n =>
        eq_trans
@@ -4272,7 +4290,8 @@ exact (fun n =>
             (eq_sym
                (compSubstRen_label tau_label id
                   (funcomp (ren_label id) tau_label) (fun x => eq_refl)
-                  (sigma n))) (ap (ren_label id) (Eq n)))).
+                  (sigma n)))
+            (ap (ren_label id) (Eq n)))).
 Qed.
 
 Lemma up_subst_subst_ty_ty {k : nat} {l_label l_ty : nat}
@@ -4282,7 +4301,8 @@ Lemma up_subst_subst_ty_ty {k : nat} {l_label l_ty : nat}
   (Eq : forall x, funcomp (subst_ty tau_label tau_ty) sigma x = theta x) :
   forall x,
   funcomp (subst_ty (up_ty_label tau_label) (up_ty_ty tau_ty))
-    (up_ty_ty sigma) x = up_ty_ty theta x.
+    (up_ty_ty sigma) x =
+  up_ty_ty theta x.
 Proof.
 exact (fun n =>
        match n with
@@ -4311,7 +4331,8 @@ Lemma up_subst_subst_list_label_ty {p : nat} {k : nat} {l_label l_ty : nat}
   forall x,
   funcomp
     (subst_ty (up_list_label_label p tau_label) (up_list_label_ty p tau_ty))
-    (up_list_label_ty p sigma) x = up_list_label_ty p theta x.
+    (up_list_label_ty p sigma) x =
+  up_list_label_ty p theta x.
 Proof.
 exact (fun n =>
        eq_trans
@@ -4334,7 +4355,8 @@ Lemma up_subst_subst_list_ty_label {p : nat} {k : nat} {l_label : nat}
   (Eq : forall x, funcomp (subst_label tau_label) sigma x = theta x) :
   forall x,
   funcomp (subst_label (up_list_ty_label p tau_label))
-    (up_list_ty_label p sigma) x = up_list_ty_label p theta x.
+    (up_list_ty_label p sigma) x =
+  up_list_ty_label p theta x.
 Proof.
 exact (fun n =>
        eq_trans
@@ -4344,7 +4366,8 @@ exact (fun n =>
          (eq_trans
             (eq_sym
                (compSubstRen_label tau_label id _ (fun x => eq_sym eq_refl)
-                  (sigma n))) (ap (ren_label id) (Eq n)))).
+                  (sigma n)))
+            (ap (ren_label id) (Eq n)))).
 Qed.
 
 Lemma up_subst_subst_list_ty_ty {p : nat} {k : nat} {l_label l_ty : nat}
@@ -4354,7 +4377,8 @@ Lemma up_subst_subst_list_ty_ty {p : nat} {k : nat} {l_label l_ty : nat}
   (Eq : forall x, funcomp (subst_ty tau_label tau_ty) sigma x = theta x) :
   forall x,
   funcomp (subst_ty (up_list_ty_label p tau_label) (up_list_ty_ty p tau_ty))
-    (up_list_ty_ty p sigma) x = up_list_ty_ty p theta x.
+    (up_list_ty_ty p sigma) x =
+  up_list_ty_ty p theta x.
 Proof.
 exact (fun n =>
        eq_trans
@@ -5207,8 +5231,8 @@ Ltac asimpl := check_no_evars;
                   Up_tm_tm, Up_tm, up_tm, Subst_tm, Subst2, subst2,
                   VarInstance_ty, Var, ids, Ren_ty, Ren2, ren2, Up_label_ty,
                   Up_ty, up_ty, Up_ty_label, Up_label, up_label, Up_ty_ty,
-                  Up_ty, up_ty, Subst_ty, Subst2, subst2 in *; asimpl';
-                minimize.
+                  Up_ty, up_ty, Subst_ty, Subst2, subst2 in *;
+                asimpl'; minimize.
 
 Tactic Notation "asimpl" "in" hyp(J) := revert J; asimpl; intros J.
 
@@ -5301,7 +5325,7 @@ Arguments app {n_label n_tm}.
 
 Arguments zero {n_label n_tm}.
 
-Arguments op {n_label n_tm}.
+Arguments Op {n_label n_tm}.
 
 Arguments l_lam {n_label n_tm}.
 
