Owl/owl_typing.v
@@ -10,41 +10,6 @@ From Coq Require Import Arith.Arith.
 (* d for type variables in scope  *)
 (* m for term variables in scope  *)
 
-Require Import FunctionalExtensionality.
-
-(* Probablity code *)
-Inductive Dist A :=
-    | Ret : A -> Dist A
-    | Flip : ( bool -> Dist A) -> Dist A.
-
-Check Ret.
-
-Arguments Ret [A].
-Arguments Flip [A].
-
-Fixpoint bind {A B} (c : Dist A) (k : A -> Dist B) : Dist B :=
-    match c with 
-    | Ret x => k x
-    | Flip f => Flip (fun x => bind (f x) k)
-    end.
-
-Definition flip : Dist bool := Flip (fun x => Ret x).
-
-Notation "x <- c1 ;; c2" := (bind c1 (fun x => c2))
-  (at level 100, c1 at next level, right associativity).
-
-Notation "'ret' x" := (Ret x)
-  (at level 100).
-
-Lemma bindA {A B C} (c : Dist A) (k : A -> Dist B) (k' : B -> Dist C) : 
-    (y <- (x <- c ;; k x);; k' y) =
-    (x <- c ;; y <- k x ;; k' y).
-    induction c; simpl.
-    auto.
-    f_equal.
-    apply functional_extensionality; intro; eauto.
-Qed.
-
 (* Example: *)
 
 Axiom foo : list nat -> Dist nat.
